


{{< include ../math.qmd >}} 






$$
\Var(y_i-\bar{y})=\Var(y_i-\frac1n\sum y_j)=\Var(\frac{n-1}{n}y_i-\sum_{j\neq i}\frac1ny_j)=\frac{(n-1)^2}{n^2}\sigma^2+\frac{n-1}{n^2}\sigma^2=\frac{n-1}{n}\sigma^2.
$$


Since $\sum_i (x_i-\bar{x})=\sum_i (y_i-\bar{y})=0$, we have
$$
\sum_i (x_i-\bar{x})\bar{x}=\sum_i (x_i-\bar{x})\bar{y}=\sum_i (y_i-\bar{y})\bar{x}=\sum_i (y_i-\bar{y})\bar{y}=0.
$$



$$
\begin{split}
\Var(S_{xy})&=\Var\qty[\sum_i (x_i-\bar{x})(y_i-\bar{y})]=\Var\qty[\sum_i (x_i-\bar{x})y_i-\sum_i (x_i-\bar{x})\bar{y}]=\Var\qty[\sum_i (x_i-\bar{x})y_i]\\
&=\sum(x_i-\bar{x})^2\Var(y_i)=\sum(x_i-\bar{x})^2\sigma^2=S_{xx}\sigma^2.
\end{split}
$$


$$
\Var(\hat{\beta}_1)=\frac{1}{S_{xx}^2}\Var(S_{xy})=\frac{1}{S_{xx}^2}\Var\qty[\sum x_i(y_i-\bar{y})]=\frac{1}{S_{xx}^2}S_{xx}\sigma^2=\frac{\sigma^2}{S_{xx}}.
$$




::: {#thm-}
## Uncorrelation 
$\hat{\beta}_0$ and $\bar y$ are uncorrelated.
:::

::: {.proof}
$$
\begin{split}
\Cov(\hat{\beta}_1,\bar{y})=&\Cov\qty(\frac{1}{S_{xx}}\sum_i(x_i-\bar x)(y_i-\bar y), \sum\frac{1}{n} y_j)=\sum_{i,j}\frac{(x_i-\bar x)}{nS_{xx}}\Cov(y_i,y_j)\\
=&\sum_{i}\frac{(x_i-\bar x)}{nS_{xx}}\sigma^2=0.
\end{split}
$$
Since $\hat{\beta}_1$ and $\bar y$ are both normal, the uncorrelation implies that they are also indepedent.
:::


$$
\begin{split}
\Var(\hat{\beta}_0)&=\Var\qty(\bar y-\hat{\beta}_1\bar x)=\Var(\bar y)+\bar{x}^2\Var(\hat{\beta}_1)=\frac{\sigma^2}{n}+\bar x^2\frac{\sigma^2}{nS_{xx}}=\qty(\frac{1}{n}+\frac{\bar x^2}{nS_{xx}})\sigma^2.
\end{split}
$$



$$
\begin{split}
\Exp\qty(y_i-\hat{y}_i)^2&=\Exp\qty(y_i-\hat{\beta}_0-\hat{\beta}_1x_i)^2
\end{split}
$$

$$
\Exp\qty(\sum(y_i-\hat{y}_i)^2)=\Exp\qty(\sum(y_i-\bar{y}_i)^2) - \Exp(S_{xy}^2) =(n-2)\sigma^2.
$$

$$
\Var(y_i-\bar y)=\Var\qty(y_i-\sum\frac1n y_j)=\Var\qty(\sum_{j\neq i}\qty(-\frac1n)y_j+\frac{n-1}n y_i)=\sum_{j\neq i}\frac1{n^2}\Var(y_j)+\frac{(n-1)^2}{n^2}\Var{y_i}=\frac{n-1}{n}\sigma^2.
$$

$$
\Exp\qty(y_i-\bar y)=\Exp(y_i)-\Exp(\bar y)=\beta_0+\beta_1x_i-\qty(\beta_0+\beta_1\bar x)=\beta_1(x_i-\bar x).
$$

$$
\sum\qty(\Exp\qty(y_i-\bar y))^2=\sum\qty(\Exp(y_i)-\Exp(\bar y))^2=\sum\qty(\beta_0+\beta_1x_i-\qty(\beta_0+\beta_1\bar x))^2=\sum\qty(\beta_1(x_i-\bar x))^2=\beta_1^2S_{xx}.
$$

$$
\begin{split}
\Exp\qty(\sum(y_i-\bar{y}_i)^2)&=\sum\Exp\qty((y_i-\bar{y})^2)=\sum\qty(\Exp\qty(y_i-\bar{y}))^2+\sum\Var(y_i-\bar y) =\beta_1^2S_{xx}+(n-1)\sigma^2.
\end{split}
$$



$$ 
\begin{split}
\Exp(S_{xy})&=\Exp\qty(\sum(x_i-\bar x)(y_i-\bar y))=\Exp\qty(\sum(x_i-\bar x)y_i)=\sum(x_i-\bar x)E(y_i)\\
&=\sum(x_i-\bar x)(\beta_0+\beta_1x_i)=\sum(x_i-\bar x)\beta_1x_i=\beta_1\sum(x_i-\bar x)x_i=\beta_1\sum(x_i-\bar x)^2\\
&=\beta_1S_{xx}.
\end{split}
$$



$$ 
\begin{split}
\Exp(S_{xy}^2)&=\qty(\Exp(S_{xy}))^2+\Var(S_{xy})=\beta_1^2S_{xx}^2+S_{xx}\sigma^2.
\end{split}
$$

$$ 
\begin{split}
\Exp(\frac{S_{xy}^2}{S_{xx}})&=\frac{1}{S_{xx}}\beta_1^2S_{xx}^2+\frac{1}{S_{xx}}S_{xx}\sigma^2=\beta_1^2S_{xx}+\sigma^2.
\end{split}
$$


1. $\Exp(S_{xy})=\beta_1S_{xx}$.
2. $\Var(S_{xy})=S_{xx}\sigma^2$.
3. $\Exp(S_{yy})=(n-2)\sigma^2$.
<!-- 4. $\Var(S_{yy})=(n-2)\sigma^2$. -->


1. $\Exp(S_{xy})$
2. $\Var(\S_{xy})$
3. $SST=SSE+SSR$
4. $\Exp(SST)$
5. $\Exp(SSR)$
6. $\Exp(SSE)$
7. $\Var(SST)$
8. $\Var(SSR)$
9. $\Var(SSR)$

